PREFIX : <http://resource.geoscience.gov.au/classifier/ggic/tenementtype/>
PREFIX cs: <http://resource.geoscience.gov.au/classifierscheme/ggic/2016.01/tenementtype>
PREFIX ggic-al: <http://resource.geoscience.gov.au/classifier/ggic/AbbreviatedLabel>
PREFIX ggic-lhk: <http://resource.geoscience.gov.au/classifier/ggic/LocalHierarchyKey>
PREFIX owl: <http://www.w3.org/2002/07/owl#>
PREFIX rdfs: <http://www.w3.org/2000/01/rdf-schema#>
PREFIX schema: <https://schema.org/>
PREFIX skos: <http://www.w3.org/2004/02/skos/core#>
PREFIX xsd: <http://www.w3.org/2001/XMLSchema#>

<http://resource.geoscience.gov.au/classifier/ggic/tenementtype>
    a skos:Collection ;
    rdfs:isDefinedBy cs: ;
    skos:definition "All the Concepts in this ConceptScheme"@en ;
    skos:historyNote "Defined in this vocabulary as a flat listing of all its Concepts" ;
    skos:inScheme cs: ;
    skos:member
        :Christmas-Island-mining-lease ,
        :ancillary-mining-licence ,
        :assessment-lease ,
        :assessment-lease-private-mineral ,
        :christmas-island-exploration-licence ,
        :coal-mining-lease ,
        :commonwealth-exploration-licence ,
        :consolidated-mining-lease ,
        :continental-shelf-licence ,
        :dredging-lease ,
        :exploration ,
        :exploration-licence ,
        :exploration-licence-application ,
        :exploration-licence-in-retention ,
        :exploration-licence-offshore ,
        :exploration-licence-private-mineral ,
        :exploration-licence-substitution ,
        :exploration-permit ,
        :exploration-permit-for-coal ,
        :exploration-permit-for-minerals ,
        :exploration-permit-special ,
        :exploration-prospecting-lease ,
        :exploration-release-area ,
        :extractive-mineral-exploration-licence ,
        :extractive-mineral-lease ,
        :extractive-mineral-permit ,
        :fossicking-area ,
        :general-purpose-lease ,
        :general-purpose-lease-sa ,
        :gold-fossicking-area ,
        :gold-lease ,
        :lease ,
        :licence ,
        :licence-to-treat-tailings ,
        :mineral-claim-converted-to-lease ,
        :mineral-claim-exploration ,
        :mineral-claim-production ,
        :mineral-development-licence ,
        :mineral-lease ,
        :mineral-lease-sa ,
        :mining-claim ,
        :mining-lease ,
        :mining-lease-SA ,
        :mining-licence ,
        :mining-mineral-owner-lease ,
        :mining-permit ,
        :mining-purposes-lease ,
        :miscellaneous-licence ,
        :miscellaneous-licence-sa ,
        :miscellaneous-purposes-licence ,
        :offshore-exploration-licence ,
        :offshore-mineral-licence ,
        :offshore-mining-licence ,
        :offshore-retention-licence ,
        :offshore-special-purpose-consents ,
        :private-lands-lease ,
        :private-lands-mining-purposes-lease ,
        :private-mine ,
        :private-mining-operation ,
        :production ,
        :production-licence ,
        :prospecting-licence ,
        :prospecting-permit ,
        :retention-lease ,
        :retention-licence ,
        :special-crown-private-lands-lease ,
        :special-exploration-licence ,
        :special-lease ,
        :special-mining-lease ,
        :special-purpose-mining-permit ,
        :temporary-reserve ,
        :tourist-mining-authority ,
        :work-authority ;
    skos:prefLabel "Tenement Type - All Concepts"@en ;
.

:Christmas-Island-mining-lease
    a skos:Concept ;
    skos:historyNote "WA"@en ;
    rdfs:isDefinedBy cs: ;
    skos:broader :production ;
    skos:definition "WA -"@en ;
    skos:inScheme cs: ;
    skos:notation "02.02"^^ggic-lhk: ;
    skos:prefLabel "Christmas Island mining lease"@en ;
.

:ancillary-mining-licence
    a skos:Concept ;
    skos:historyNote "NZ"@en ;
    rdfs:isDefinedBy cs: ;
    skos:broader :production ;
    skos:definition "NZ -"@en ;
    skos:inScheme cs: ;
    skos:notation "02.01"^^ggic-lhk: ;
    skos:prefLabel "ancillary mining licence"@en ;
.

:assessment-lease
    a skos:Concept ;
    skos:historyNote "NSW"@en ;
    rdfs:isDefinedBy cs: ;
    skos:broader :exploration ;
    skos:definition "NSW -"@en ;
    skos:inScheme cs: ;
    skos:notation
        "AL"^^ggic-al: ,
        "01.01"^^ggic-lhk: ;
    skos:prefLabel "assessment lease"@en ;
.

:assessment-lease-private-mineral
    a skos:Concept ;
    skos:historyNote "NSW"@en ;
    rdfs:isDefinedBy cs: ;
    skos:broader :exploration ;
    skos:definition "NSW -"@en ;
    skos:inScheme cs: ;
    skos:notation
        "A(MO)L"^^ggic-al: ,
        "01.02"^^ggic-lhk: ;
    skos:prefLabel "assessment lease (private mineral)"@en ;
.

:christmas-island-exploration-licence
    a skos:Concept ;
    skos:historyNote "WA"@en ;
    rdfs:isDefinedBy cs: ;
    skos:broader :exploration ;
    skos:definition "WA -"@en ;
    skos:inScheme cs: ;
    skos:notation "01.03"^^ggic-lhk: ;
    skos:prefLabel "Christmas Island exploration licence"@en ;
.

:coal-mining-lease
    a skos:Concept ;
    skos:historyNote "WA"@en ;
    rdfs:isDefinedBy cs: ;
    skos:broader :production ;
    skos:definition "WA - Mining lease specifically for coal under repealed 1904 Act."@en ;
    skos:inScheme cs: ;
    skos:notation "02.03"^^ggic-lhk: ;
    skos:prefLabel "coal mining lease"@en ;
.

:commonwealth-exploration-licence
    a skos:Concept ;
    skos:historyNote "WA"@en ;
    rdfs:isDefinedBy cs: ;
    skos:broader :exploration ;
    skos:definition "WA -"@en ;
    skos:inScheme cs: ;
    skos:notation "01.04"^^ggic-lhk: ;
    skos:prefLabel "Commonwealth exploration licence"@en ;
.

:consolidated-mining-lease
    a skos:Concept ;
    skos:historyNote "NSW"@en ;
    rdfs:isDefinedBy cs: ;
    skos:broader :production ;
    skos:definition "NSW -"@en ;
    skos:inScheme cs: ;
    skos:notation
        "CML"^^ggic-al: ,
        "02.04"^^ggic-lhk: ;
    skos:prefLabel "consolidated mining lease"@en ;
.

:continental-shelf-licence
    a skos:Concept ;
    skos:historyNote "NZ"@en ;
    rdfs:isDefinedBy cs: ;
    skos:broader :exploration ;
    skos:definition "NZ -"@en ;
    skos:inScheme cs: ;
    skos:notation "01.05"^^ggic-lhk: ;
    skos:prefLabel "continental shelf licence"@en ;
.

:dredging-lease
    a skos:Concept ;
    skos:historyNote "NSW"@en ;
    rdfs:isDefinedBy cs: ;
    skos:broader :production ;
    skos:definition "NSW -"@en ;
    skos:inScheme cs: ;
    skos:notation
        "DL"^^ggic-al: ,
        "02.05"^^ggic-lhk: ;
    skos:prefLabel "dredging lease"@en ;
.

:exploration-licence
    a skos:Concept ;
    skos:historyNote "NSW, TAS, VIC, WA, SA, NT"@en ;
    rdfs:isDefinedBy cs: ;
    skos:broader :exploration ;
    skos:definition "TAS - Standard exploration tenement type for all commodities (Categories 1 to 6). VIC - http://www.austlii.edu.au/au/legis/vic/consol_act/mrda1990432/s13.html. WA - Block based system; max 70 blocks; term 5 years plus 2 extensions; surrender 50%; 100 tonnes of material."@en ;
    skos:inScheme cs: ;
    skos:notation
        "EL"^^ggic-al: ,
        "01.06"^^ggic-lhk: ;
    skos:prefLabel "exploration licence"@en ;
.

:exploration-licence-application
    a skos:Concept ;
    skos:historyNote "SA"@en ;
    rdfs:isDefinedBy cs: ;
    skos:broader :exploration ;
    skos:definition "SA - Application for an Exploration Licence."@en ;
    skos:inScheme cs: ;
    skos:notation
        "ELA"^^ggic-al: ,
        "01.07"^^ggic-lhk: ;
    skos:prefLabel "exploration licence application"@en ;
.

:exploration-licence-in-retention
    a skos:Concept ;
    skos:historyNote "NT"@en ;
    rdfs:isDefinedBy cs: ;
    skos:altLabel "retention licence"@en ;
    skos:broader :exploration ;
    skos:definition "NT - Licence to carry out feasibility study or retain ore body not economically viable. See also 'retention licence' used by other jurisdictions."@en ;
    skos:inScheme cs: ;
    skos:notation
        "ELR"^^ggic-al: ,
        "01.11"^^ggic-lhk: ;
    skos:prefLabel "exploration licence in retention"@en ;
.

:exploration-licence-offshore
    a skos:Concept ;
    skos:historyNote "WA"@en ;
    rdfs:isDefinedBy cs: ;
    skos:broader :exploration ;
    skos:definition "WA -"@en ;
    skos:inScheme cs: ;
    skos:notation "01.08"^^ggic-lhk: ;
    skos:prefLabel "exploration licence offshore"@en ;
.

:exploration-licence-private-mineral
    a skos:Concept ;
    skos:historyNote "NSW"@en ;
    rdfs:isDefinedBy cs: ;
    skos:broader :exploration ;
    skos:definition "NSW -"@en ;
    skos:inScheme cs: ;
    skos:notation
        "E(MO)L"^^ggic-al: ,
        "01.09"^^ggic-lhk: ;
    skos:prefLabel "exploration licence (private mineral)"@en ;
.

:exploration-licence-substitution
    a skos:Concept ;
    skos:historyNote "NT"@en ;
    rdfs:isDefinedBy cs: ;
    skos:broader :exploration ;
    skos:definition "NT - Replacement exploration licence when amalgamating two or more ELs after expiry of original grant/allowed renewal periods. No longer active title type under the MTA"@en ;
    skos:inScheme cs: ;
    skos:notation
        "SEL"^^ggic-al: ,
        "01.10"^^ggic-lhk: ;
    skos:prefLabel "exploration licence - substitution"@en ;
.

:exploration-permit
    a skos:Concept ;
    skos:historyNote "NZ"@en ;
    rdfs:isDefinedBy cs: ;
    skos:broader :exploration ;
    skos:definition "NZ -"@en ;
    skos:inScheme cs: ;
    skos:notation "01.12"^^ggic-lhk: ;
    skos:prefLabel "exploration permit"@en ;
.

:exploration-permit-for-coal
    a skos:Concept ;
    skos:historyNote "QLD"@en ;
    rdfs:isDefinedBy cs: ;
    skos:broader :exploration ;
    skos:definition "QLD - Standard exploration permit for coal which allows for overlap with EPM or EPS."@en ;
    skos:inScheme cs: ;
    skos:notation
        "EPC"^^ggic-al: ,
        "01.13"^^ggic-lhk: ;
    skos:prefLabel "exploration permit for coal"@en ;
.

:exploration-permit-for-minerals
    a skos:Concept ;
    skos:historyNote "QLD"@en ;
    rdfs:isDefinedBy cs: ;
    skos:broader :exploration ;
    skos:definition "QLD - Standard exploration permit for minerals which allows for overlap with EPC and EPS."@en ;
    skos:inScheme cs: ;
    skos:notation
        "EPM"^^ggic-al: ,
        "01.14"^^ggic-lhk: ;
    skos:prefLabel "exploration permit for minerals"@en ;
.

:exploration-permit-special
    a skos:Concept ;
    skos:historyNote "QLD"@en ;
    rdfs:isDefinedBy cs: ;
    skos:broader :exploration ;
    skos:definition "QLD - Special exploration permit for minerals which allows for overlap with EPM by mutual agreement with EPM holder where minerals sought are mutually exclusive."@en ;
    skos:inScheme cs: ;
    skos:notation
        "EPS"^^ggic-al: ,
        "01.15"^^ggic-lhk: ;
    skos:prefLabel "exploration permit special"@en ;
.

:exploration-prospecting-lease
    a skos:Concept ;
    skos:historyNote "NSW"@en ;
    rdfs:isDefinedBy cs: ;
    skos:broader :exploration ;
    skos:definition "NSW -"@en ;
    skos:inScheme cs: ;
    skos:notation
        "EPL"^^ggic-al: ,
        "01.16"^^ggic-lhk: ;
    skos:prefLabel "exploration prospecting lease"@en ;
.

:exploration-release-area
    a skos:Concept ;
    skos:historyNote "SA"@en ;
    rdfs:isDefinedBy cs: ;
    skos:broader :exploration ;
    skos:definition "missing"@en ;
    skos:inScheme cs: ;
    skos:notation
        "ERA"^^ggic-al: ,
        "01.17"^^ggic-lhk: ;
    skos:prefLabel "exploration release area"@en ;
.

:extractive-mineral-exploration-licence
    a skos:Concept ;
    skos:historyNote "NT"@en ;
    rdfs:isDefinedBy cs: ;
    skos:broader :exploration ;
    skos:definition "NT - To explore for extractive minerals"@en ;
    skos:inScheme cs: ;
    skos:notation
        "EMEL"^^ggic-al: ,
        "01.18"^^ggic-lhk: ;
    skos:prefLabel "extractive mineral exploration licence"@en ;
.

:extractive-mineral-lease
    a skos:Concept ;
    skos:historyNote "SA, NT"@en ;
    rdfs:isDefinedBy cs: ;
    skos:broader :production ;
    skos:definition "SA - An EML entitles the lessee to carry out mining operations specified in the lease for the recovery of extractive minerals. NT - To mine for extractive minerals and/or erect infrastructure"@en ;
    skos:inScheme cs: ;
    skos:notation
        "EML"^^ggic-al: ,
        "02.06"^^ggic-lhk: ;
    skos:prefLabel "extractive mineral lease"@en ;
.

:extractive-mineral-permit
    a skos:Concept ;
    skos:historyNote "NT"@en ;
    rdfs:isDefinedBy cs: ;
    skos:broader :production ;
    skos:definition "NT - A permit to extract, remove, store or process extractive minerals"@en ;
    skos:inScheme cs: ;
    skos:notation
        "EMP"^^ggic-al: ,
        "02.07"^^ggic-lhk: ;
    skos:prefLabel "extractive mineral permit"@en ;
.

:fossicking-area
    a skos:Concept ;
    skos:historyNote "NT"@en ;
    rdfs:isDefinedBy cs: ;
    skos:broader :exploration ;
    skos:definition "NT - Declared areas for fossicking"@en ;
    skos:inScheme cs: ;
    skos:notation
        "FA"^^ggic-al: ,
        "01.19"^^ggic-lhk: ;
    skos:prefLabel "fossicking area (s.131)"@en ;
.

:general-purpose-lease
    a skos:Concept ;
    skos:historyNote "WA"@en ;
    rdfs:isDefinedBy cs: ;
    skos:broader :production ;
    skos:definition "WA - Lease not specifically for mineral extraction. Linked to mining opreations for purposes of operating machinery and depositing tailings."@en ;
    skos:inScheme cs: ;
    skos:notation "02.08"^^ggic-lhk: ;
    skos:prefLabel "general purpose lease"@en ;
.

:general-purpose-lease-sa
    a skos:Concept ;
    skos:historyNote "WA"@en ;
    rdfs:isDefinedBy cs: ;
    skos:broader :production ;
    skos:definition "WA - Lease not specifically for mineral extraction. Linked to mining opreations for purposes of operating machinery and depositing tailings, in State Agreement area."@en ;
    skos:inScheme cs: ;
    skos:notation "02.09"^^ggic-lhk: ;
    skos:prefLabel "general purpose lease S.A."@en ;
.

:gold-fossicking-area
    a skos:Concept ;
    skos:historyNote "NZ"@en ;
    rdfs:isDefinedBy cs: ;
    skos:broader :exploration ;
    skos:definition "NZ -"@en ;
    skos:inScheme cs: ;
    skos:notation "01.20"^^ggic-lhk: ;
    skos:prefLabel "gold fossicking area"@en ;
.

:gold-lease
    a skos:Concept ;
    skos:historyNote "NSW"@en ;
    rdfs:isDefinedBy cs: ;
    skos:broader :production ;
    skos:definition "NSW -"@en ;
    skos:inScheme cs: ;
    skos:notation
        "GL"^^ggic-al: ,
        "02.10"^^ggic-lhk: ;
    skos:prefLabel "gold lease"@en ;
.

:lease
    a skos:Concept ;
    skos:historyNote "TAS"@en ;
    rdfs:isDefinedBy cs: ;
    skos:broader :production ;
    skos:definition "TAS -"@en ;
    skos:inScheme cs: ;
    skos:notation "02.11"^^ggic-lhk: ;
    skos:prefLabel "lease"@en ;
.

:licence
    a skos:Concept ;
    skos:historyNote "TAS"@en ;
    rdfs:isDefinedBy cs: ;
    skos:broader :exploration ;
    skos:definition "TAS -"@en ;
    skos:inScheme cs: ;
    skos:notation "01.21"^^ggic-lhk: ;
    skos:prefLabel "licence"@en ;
.

:licence-to-treat-tailings
    a skos:Concept ;
    skos:historyNote "WA"@en ;
    rdfs:isDefinedBy cs: ;
    skos:broader :production ;
    skos:definition "WA - Mining tenement under the repealed 1904 Act."@en ;
    skos:inScheme cs: ;
    skos:notation "02.12"^^ggic-lhk: ;
    skos:prefLabel "licence to treat tailings"@en ;
.

:mineral-claim-converted-to-lease
    a skos:Concept ;
    skos:historyNote "NSW"@en ;
    rdfs:isDefinedBy cs: ;
    skos:broader :production ;
    skos:definition "NSW -"@en ;
    skos:inScheme cs: ;
    skos:notation
        "M(C)L"^^ggic-al: ,
        "02.13"^^ggic-lhk: ;
    skos:prefLabel "mineral claim converted to lease"@en ;
.

:mineral-claim-exploration
    a skos:Concept ;
    skos:historyNote "WA"@en ;
    rdfs:isDefinedBy cs: ;
    skos:broader :exploration ;
    skos:definition "WA -"@en ;
    skos:inScheme cs: ;
    skos:notation "01.22"^^ggic-lhk: ;
    skos:prefLabel "mineral claim (exploration)"@en ;
.

:mineral-claim-production
    a skos:Concept ;
    skos:historyNote "SA, NT"@en ;
    rdfs:isDefinedBy cs: ;
    skos:broader :production ;
    skos:definition "SA - An MC provides an exclusive right for 12 months to prospect for minerals within the claim area (conditions apply). NT - Small scale mining or exploration up to 40 Ha under the Mining Act. Not an active title type under the MTA and are in process of being converted to appropriate title type."@en ;
    skos:inScheme cs: ;
    skos:notation
        "MC"^^ggic-al: ,
        "02.16"^^ggic-lhk: ;
    skos:prefLabel "mineral claim (production)"@en ;
.

:mineral-development-licence
    a skos:Concept ;
    skos:historyNote "QLD"@en ;
    rdfs:isDefinedBy cs: ;
    skos:broader :exploration ;
    skos:definition "QLD - A holding permit for coal or minerals which allows further exploration and testing within limits."@en ;
    skos:inScheme cs: ;
    skos:notation
        "MDL"^^ggic-al: ,
        "01.23"^^ggic-lhk: ;
    skos:prefLabel "mineral development licence"@en ;
.

:mineral-lease
    a skos:Concept ;
    skos:historyNote "SA, WA, NT"@en ;
    rdfs:isDefinedBy cs: ;
    skos:broader :production ;
    skos:definition "SA - An ML entitles the lessee to carry out mining operations specified in the lease for the recovery of minerals other than extractive minerals. WA - Mining tenement under the repealed 1904 Act. NT - To mine for minerals, and/or erect infrastructures."@en ;
    skos:inScheme cs: ;
    skos:notation
        "ML"^^ggic-al: ,
        "02.14"^^ggic-lhk: ;
    skos:prefLabel "mineral lease"@en ;
.

:mineral-lease-sa
    a skos:Concept ;
    skos:historyNote "WA"@en ;
    rdfs:isDefinedBy cs: ;
    skos:broader :production ;
    skos:definition "WA - Special Agreement Act mineral lease."@en ;
    skos:inScheme cs: ;
    skos:notation "02.15"^^ggic-lhk: ;
    skos:prefLabel "mineral lease S.A."@en ;
.

:mining-claim
    a skos:Concept ;
    skos:historyNote "QLD"@en ;
    rdfs:isDefinedBy cs: ;
    skos:broader :production ;
    skos:definition "QLD - Small scale mining activity commonly used for gemstones, opals and sometimes gold; Limited area and conditions on production methods"@en ;
    skos:inScheme cs: ;
    skos:notation
        "MC"^^ggic-al: ,
        "02.17"^^ggic-lhk: ;
    skos:prefLabel "mining claim"@en ;
.

:mining-lease
    a skos:Concept ;
    skos:historyNote "NSW, TAS, WA, QLD"@en ;
    rdfs:isDefinedBy cs: ;
    skos:broader :production ;
    skos:definition "TAS - Standard mineral extraction lease (for mineral categories 1,2,3 and 5). WA - Tenement on which there is an identified mineral resource for mining. Term 21 years + renewal."@en ;
    skos:inScheme cs: ;
    skos:notation
        "ML"^^ggic-al: ,
        "02.18"^^ggic-lhk: ;
    skos:prefLabel "mining lease"@en ;
.

:mining-lease-SA
    a skos:Concept ;
    skos:historyNote "WA"@en ;
    rdfs:isDefinedBy cs: ;
    skos:broader :production ;
    skos:definition "WA - Max area 200 ha,term 4 years can extract 500 tonnes of material"@en ;
    skos:inScheme cs: ;
    skos:notation "02.19"^^ggic-lhk: ;
    skos:prefLabel "mining lease S.A."@en ;
.

:mining-licence
    a skos:Concept ;
    skos:historyNote "VIC, NZ"@en ;
    rdfs:isDefinedBy cs: ;
    skos:broader :production ;
    skos:definition "VIC - http://www.austlii.edu.au/au/legis/vic/consol_act/mrda1990432/s14.html"@en ;
    skos:inScheme cs: ;
    skos:notation "02.20"^^ggic-lhk: ;
    skos:prefLabel "mining licence"@en ;
.

:mining-mineral-owner-lease
    a skos:Concept ;
    skos:historyNote "NSW"@en ;
    rdfs:isDefinedBy cs: ;
    skos:broader :production ;
    skos:definition "NSW -"@en ;
    skos:inScheme cs: ;
    skos:notation
        "M(MO)L"^^ggic-al: ,
        "02.21"^^ggic-lhk: ;
    skos:prefLabel "mining (mineral owner) lease"@en ;
.

:mining-permit
    a skos:Concept ;
    skos:historyNote "NZ"@en ;
    rdfs:isDefinedBy cs: ;
    skos:broader :production ;
    skos:definition "NZ -"@en ;
    skos:inScheme cs: ;
    skos:notation "02.22"^^ggic-lhk: ;
    skos:prefLabel "mining permit"@en ;
.

:mining-purposes-lease
    a skos:Concept ;
    skos:historyNote "NSW"@en ;
    rdfs:isDefinedBy cs: ;
    skos:broader :production ;
    skos:definition "NSW -"@en ;
    skos:inScheme cs: ;
    skos:notation
        "MPL"^^ggic-al: ,
        "02.23"^^ggic-lhk: ;
    skos:prefLabel "mining purposes lease"@en ;
.

:miscellaneous-licence
    a skos:Concept ;
    skos:historyNote "WA"@en ;
    rdfs:isDefinedBy cs: ;
    skos:broader :production ;
    skos:definition "WA - Lease not specifically for mineral extraction. An ancilliary tenement to a mining lease for the purposes of infrastructure such as roads, pipelines etc."@en ;
    skos:inScheme cs: ;
    skos:notation "02.24"^^ggic-lhk: ;
    skos:prefLabel "miscellaneous licence"@en ;
.

:miscellaneous-licence-sa
    a skos:Concept ;
    skos:historyNote "WA"@en ;
    rdfs:isDefinedBy cs: ;
    skos:broader :production ;
    skos:definition "WA - Lease not specifically for mineral extraction. An ancilliary tenement to a mining lease for the purposes of infrastructure such as roads, pipelines etc, under a Special Agreement Act."@en ;
    skos:inScheme cs: ;
    skos:notation "02.25"^^ggic-lhk: ;
    skos:prefLabel "miscellaneous licence S.A."@en ;
.

:miscellaneous-purposes-licence
    a skos:Concept ;
    skos:historyNote "SA"@en ;
    rdfs:isDefinedBy cs: ;
    skos:broader :production ;
    skos:definition "SA - An MPL may be granted for any purpose ancillary to the conduct of mining operations, for example an operating plant, drainage or an access road."@en ;
    skos:inScheme cs: ;
    skos:notation
        "MPL"^^ggic-al: ,
        "02.26"^^ggic-lhk: ;
    skos:prefLabel "miscellaneous purposes licence"@en ;
.

:offshore-exploration-licence
    a skos:Concept ;
    skos:historyNote "NT"@en ;
    rdfs:isDefinedBy cs: ;
    skos:broader :exploration ;
    skos:definition "NT - Offshore Waters [Applications of Territory Laws] Act 1994. To explore for minerals outside of the 3 nautical mile"@en ;
    skos:inScheme cs: ;
    skos:notation
        "OEL"^^ggic-al: ,
        "01.24"^^ggic-lhk: ;
    skos:prefLabel "offshore exploration licence"@en ;
.

:offshore-mineral-licence
    a skos:Concept ;
    skos:historyNote "TAS"@en ;
    rdfs:isDefinedBy cs: ;
    skos:broader :exploration ;
    skos:definition "TAS -"@en ;
    skos:inScheme cs: ;
    skos:notation "01.25"^^ggic-lhk: ;
    skos:prefLabel "offshore mineral licence"@en ;
.

:offshore-mining-licence
    a skos:Concept ;
    skos:historyNote "NT"@en ;
    rdfs:isDefinedBy cs: ;
    skos:broader :production ;
    skos:definition "NT - Off-shore Waters [Application of Territory Laws] Act 1994 To mine for minerals outside the 3 nautical mile"@en ;
    skos:inScheme cs: ;
    skos:notation
        "OML"^^ggic-al: ,
        "02.27"^^ggic-lhk: ;
    skos:prefLabel "offshore mining licence"@en ;
.

:offshore-retention-licence
    a skos:Concept ;
    skos:historyNote "NT"@en ;
    rdfs:isDefinedBy cs: ;
    skos:broader :exploration ;
    skos:definition "NT - Off-shore Waters [Application of Territory Laws] Act 1994"@en ;
    skos:inScheme cs: ;
    skos:notation
        "ORL"^^ggic-al: ,
        "01.26"^^ggic-lhk: ;
    skos:prefLabel "offshore retention licence"@en ;
.

:offshore-special-purpose-consents
    a skos:Concept ;
    skos:historyNote "NT"@en ;
    rdfs:isDefinedBy cs: ;
    skos:broader :exploration ;
    skos:definition "NT - A special purpose consent authorises the holder to carry out either scientific investigations, a reconnaissance survey or collect a small amount of minerals. Actually a title under the Commonwealth Offshore Minerals Act, but each state were to use as model for within 3 mile limit."@en ;
    skos:inScheme cs: ;
    skos:notation
        "OSPC"^^ggic-al: ,
        "01.27"^^ggic-lhk: ;
    skos:prefLabel "offshore special purpose consents"@en ;
.

:private-lands-lease
    a skos:Concept ;
    skos:historyNote "NSW"@en ;
    rdfs:isDefinedBy cs: ;
    skos:broader :production ;
    skos:definition "NSW -"@en ;
    skos:inScheme cs: ;
    skos:notation
        "PLL"^^ggic-al: ,
        "02.28"^^ggic-lhk: ;
    skos:prefLabel "private lands lease"@en ;
.

:private-lands-mining-purposes-lease
    a skos:Concept ;
    skos:historyNote "NSW"@en ;
    rdfs:isDefinedBy cs: ;
    skos:broader :production ;
    skos:definition "NSW -"@en ;
    skos:inScheme cs: ;
    skos:notation
        "PL(MP)L"^^ggic-al: ,
        "02.29"^^ggic-lhk: ;
    skos:prefLabel "private lands (mining purposes) lease"@en ;
.

:private-mine
    a skos:Concept ;
    skos:historyNote "SA"@en ;
    rdfs:isDefinedBy cs: ;
    skos:broader :production ;
    skos:definition "SA - tenements declared prior to the Mining Act, 1971 and are subject to specific conditions."@en ;
    skos:inScheme cs: ;
    skos:notation "02.30"^^ggic-lhk: ;
    skos:prefLabel "private mine"@en ;
.

:private-mining-operation
    a skos:Concept ;
    skos:historyNote "NZ"@en ;
    rdfs:isDefinedBy cs: ;
    skos:broader :production ;
    skos:definition "NZ -"@en ;
    skos:inScheme cs: ;
    skos:notation "02.31"^^ggic-lhk: ;
    skos:prefLabel "private mining operation"@en ;
.

:production-licence
    a skos:Concept ;
    skos:historyNote "TAS"@en ;
    rdfs:isDefinedBy cs: ;
    skos:broader :production ;
    skos:definition "TAS - for extraction of Geothermal (category 6) or onshore oil and gas (category 4)"@en ;
    skos:inScheme cs: ;
    skos:notation "02.32"^^ggic-lhk: ;
    skos:prefLabel "production licence"@en ;
.

:prospecting-licence
    a skos:Concept ;
    skos:historyNote "VIC, WA, NZ"@en ;
    rdfs:isDefinedBy cs: ;
    skos:broader :exploration ;
    skos:definition "WA - licence for prospecting, up to 200 hectares, 4 year term + 4year extension. Removal of up to 500 t of material allowed. VIC - http://www.austlii.edu.au/au/legis/vic/consol_act/mrda1990432/s14b.html"@en ;
    skos:inScheme cs: ;
    skos:notation "01.28"^^ggic-lhk: ;
    skos:prefLabel "prospecting licence"@en ;
.

:prospecting-permit
    a skos:Concept ;
    skos:historyNote "NZ, WA, QLD"@en ;
    rdfs:isDefinedBy cs: ;
    skos:broader :exploration ;
    skos:definition "QLD - Allows small scale exploration with area limits and pegging for mining applications"@en ;
    skos:inScheme cs: ;
    skos:notation "01.29"^^ggic-lhk: ;
    skos:prefLabel "prospecting permit"@en ;
.

:retention-lease
    a skos:Concept ;
    skos:historyNote "SA"@en ;
    rdfs:isDefinedBy cs: ;
    skos:broader :production ;
    skos:definition "SA - An RL entitles the lessee to retain the lease area for future mining operations where, for economic or other reasons, the lessee is justified in not proceeding immediately."@en ;
    skos:inScheme cs: ;
    skos:notation "02.33"^^ggic-lhk: ;
    skos:prefLabel "retention lease"@en ;
.

:retention-licence
    a skos:Concept ;
    skos:historyNote "TAS, VIC, WA"@en ;
    rdfs:isDefinedBy cs: ;
    skos:altLabel "exploration licence in retention"@en ;
    skos:broader :exploration ;
    skos:definition "TAS - Exploration tenement where a resource has been defined but is currently sub-economic, and requires further exploratoin before a Mining lease can be granted VIC - http://www.austlii.edu.au/au/legis/vic/consol_act/mrda1990432/s14c.html. WA - Holding title for an identified mineral resource for later mining, but is not able to be further explored or mined."@en ;
    skos:inScheme cs: ;
    skos:notation "01.30"^^ggic-lhk: ;
    skos:prefLabel "retention licence"@en ;
.

:special-crown-private-lands-lease
    a skos:Concept ;
    skos:historyNote "NSW"@en ;
    rdfs:isDefinedBy cs: ;
    skos:broader :production ;
    skos:definition "NSW -"@en ;
    skos:inScheme cs: ;
    skos:notation
        "S(C&PL)L"^^ggic-al: ,
        "02.34"^^ggic-lhk: ;
    skos:prefLabel "special (crown & private lands) lease"@en ;
.

:special-exploration-licence
    a skos:Concept ;
    skos:historyNote "TAS"@en ;
    rdfs:isDefinedBy cs: ;
    skos:broader :exploration ;
    skos:definition "TAS - Exploration tenement - larger than normal tenement to explore for new commodity types or utilise new exploration techniques. May be extended to a maximum of 10 years."@en ;
    skos:inScheme cs: ;
    skos:notation "01.31"^^ggic-lhk: ;
    skos:prefLabel "special exploration licence"@en ;
.

:special-lease
    a skos:Concept ;
    skos:historyNote "NSW"@en ;
    rdfs:isDefinedBy cs: ;
    skos:broader :production ;
    skos:definition "NSW -"@en ;
    skos:inScheme cs: ;
    skos:notation
        "SL"^^ggic-al: ,
        "02.35"^^ggic-lhk: ;
    skos:prefLabel "special lease"@en ;
.

:special-mining-lease
    a skos:Concept ;
    skos:historyNote "SA"@en ;
    rdfs:isDefinedBy cs: ;
    skos:broader :production ;
    skos:definition "SA - The tenement type SML (Special Mining Lease) relates to the Olympic Dam mine, which is administered under the Roxby Downs (Indenture Ratification) Act, 1982. There is also an historic disused tenement type SML."@en ;
    skos:inScheme cs: ;
    skos:notation "02.36"^^ggic-lhk: ;
    skos:prefLabel "special mining lease"@en ;
.

:special-purpose-mining-permit
    a skos:Concept ;
    skos:historyNote "NZ"@en ;
    rdfs:isDefinedBy cs: ;
    skos:broader :production ;
    skos:definition "NZ -"@en ;
    skos:inScheme cs: ;
    skos:notation "02.37"^^ggic-lhk: ;
    skos:prefLabel "special purpose mining permit"@en ;
.

:temporary-reserve
    a skos:Concept ;
    skos:historyNote "WA"@en ;
    rdfs:isDefinedBy cs: ;
    skos:broader :exploration ;
    skos:definition "WA - Mining tenement under the repealed 1904 Act."@en ;
    skos:inScheme cs: ;
    skos:notation "01.32"^^ggic-lhk: ;
    skos:prefLabel "temporary reserve"@en ;
.

:tourist-mining-authority
    a skos:Concept ;
    skos:historyNote "VIC"@en ;
    rdfs:isDefinedBy cs: ;
    skos:broader :exploration ;
    skos:definition "VIC - http://www.austlii.edu.au/au/legis/vic/consol_act/mrda1990432/s59.html"@en ;
    skos:inScheme cs: ;
    skos:notation "01.33"^^ggic-lhk: ;
    skos:prefLabel "tourist mining authority"@en ;
.

:work-authority
    a skos:Concept ;
    skos:historyNote "VIC"@en ;
    rdfs:isDefinedBy cs: ;
    skos:broader :production ;
    skos:definition "VIC -"@en ;
    skos:inScheme cs: ;
    skos:notation "02.38"^^ggic-lhk: ;
    skos:prefLabel "work authority"@en ;
.

:exploration
    a skos:Concept ;
    skos:historyNote "This vocabulary"@en ;
    rdfs:isDefinedBy cs: ;
    skos:definition "A tenement, permit, or licence related to mineral exploration activities."@en ;
    skos:inScheme cs: ;
    skos:narrower
        :assessment-lease ,
        :assessment-lease-private-mineral ,
        :christmas-island-exploration-licence ,
        :commonwealth-exploration-licence ,
        :continental-shelf-licence ,
        :exploration-licence ,
        :exploration-licence-application ,
        :exploration-licence-in-retention ,
        :exploration-licence-offshore ,
        :exploration-licence-private-mineral ,
        :exploration-licence-substitution ,
        :exploration-permit ,
        :exploration-permit-for-coal ,
        :exploration-permit-for-minerals ,
        :exploration-permit-special ,
        :exploration-prospecting-lease ,
        :exploration-release-area ,
        :extractive-mineral-exploration-licence ,
        :fossicking-area ,
        :gold-fossicking-area ,
        :licence ,
        :mineral-claim-exploration ,
        :mineral-development-licence ,
        :offshore-exploration-licence ,
        :offshore-mineral-licence ,
        :offshore-retention-licence ,
        :offshore-special-purpose-consents ,
        :prospecting-licence ,
        :prospecting-permit ,
        :retention-licence ,
        :special-exploration-licence ,
        :temporary-reserve ,
        :tourist-mining-authority ;
    skos:narrowerTransitive
        :assessment-lease ,
        :assessment-lease-private-mineral ,
        :christmas-island-exploration-licence ,
        :commonwealth-exploration-licence ,
        :continental-shelf-licence ,
        :exploration-licence ,
        :exploration-licence-application ,
        :exploration-licence-in-retention ,
        :exploration-licence-offshore ,
        :exploration-licence-private-mineral ,
        :exploration-licence-substitution ,
        :exploration-permit ,
        :exploration-permit-for-coal ,
        :exploration-permit-for-minerals ,
        :exploration-permit-special ,
        :exploration-prospecting-lease ,
        :exploration-release-area ,
        :extractive-mineral-exploration-licence ,
        :fossicking-area ,
        :gold-fossicking-area ,
        :licence ,
        :mineral-claim-exploration ,
        :mineral-development-licence ,
        :offshore-exploration-licence ,
        :offshore-mineral-licence ,
        :offshore-retention-licence ,
        :offshore-special-purpose-consents ,
        :prospecting-licence ,
        :prospecting-permit ,
        :retention-licence ,
        :special-exploration-licence ,
        :temporary-reserve ,
        :tourist-mining-authority ;
    skos:notation "01"^^ggic-lhk: ;
    skos:prefLabel "exploration"@en ;
    skos:topConceptOf cs: ;
.

:production
    a skos:Concept ;
    skos:historyNote "This vocabulary"@en ;
    rdfs:isDefinedBy cs: ;
    skos:definition "A tenement, permit, or licence related to mining activities or related production of mineral products."@en ;
    skos:inScheme cs: ;
    skos:narrower
        :Christmas-Island-mining-lease ,
        :ancillary-mining-licence ,
        :coal-mining-lease ,
        :consolidated-mining-lease ,
        :dredging-lease ,
        :extractive-mineral-lease ,
        :extractive-mineral-permit ,
        :general-purpose-lease ,
        :general-purpose-lease-sa ,
        :gold-lease ,
        :lease ,
        :licence-to-treat-tailings ,
        :mineral-claim-converted-to-lease ,
        :mineral-claim-production ,
        :mineral-lease ,
        :mineral-lease-sa ,
        :mining-claim ,
        :mining-lease ,
        :mining-lease-SA ,
        :mining-licence ,
        :mining-mineral-owner-lease ,
        :mining-permit ,
        :mining-purposes-lease ,
        :miscellaneous-licence ,
        :miscellaneous-licence-sa ,
        :miscellaneous-purposes-licence ,
        :offshore-mining-licence ,
        :private-lands-lease ,
        :private-lands-mining-purposes-lease ,
        :private-mine ,
        :private-mining-operation ,
        :production-licence ,
        :retention-lease ,
        :special-crown-private-lands-lease ,
        :special-lease ,
        :special-mining-lease ,
        :special-purpose-mining-permit ,
        :work-authority ;
    skos:narrowerTransitive
        :Christmas-Island-mining-lease ,
        :ancillary-mining-licence ,
        :coal-mining-lease ,
        :consolidated-mining-lease ,
        :dredging-lease ,
        :extractive-mineral-lease ,
        :extractive-mineral-permit ,
        :general-purpose-lease ,
        :general-purpose-lease-sa ,
        :gold-lease ,
        :lease ,
        :licence-to-treat-tailings ,
        :mineral-claim-converted-to-lease ,
        :mineral-claim-production ,
        :mineral-lease ,
        :mineral-lease-sa ,
        :mining-claim ,
        :mining-lease ,
        :mining-lease-SA ,
        :mining-licence ,
        :mining-mineral-owner-lease ,
        :mining-permit ,
        :mining-purposes-lease ,
        :miscellaneous-licence ,
        :miscellaneous-licence-sa ,
        :miscellaneous-purposes-licence ,
        :offshore-mining-licence ,
        :private-lands-lease ,
        :private-lands-mining-purposes-lease ,
        :private-mine ,
        :private-mining-operation ,
        :production-licence ,
        :retention-lease ,
        :special-crown-private-lands-lease ,
        :special-lease ,
        :special-mining-lease ,
        :special-purpose-mining-permit ,
        :work-authority ;
    skos:notation "02"^^ggic-lhk: ;
    skos:prefLabel "production"@en ;
    skos:topConceptOf cs: ;
.

cs:
    a skos:ConceptScheme ;
    schema:dateCreated "2015-11-26"^^xsd:date ;
    schema:creator <https://linked.data.gov.au/org/agson> ;
    schema:dateIssued "2017-09-06"^^xsd:date ;
    schema:dateModified "2024-10-16"^^xsd:date ;
    skos:historyNote "This vocabulary is expressed for the first time here" ;
    schema:publisher <https://linked.data.gov.au/org/agson> ;
    schema:citation "This vocabulary is expressed for the first time here" ;
    owl:versionInfo "v0.1"^^xsd:string ;
    skos:changeNote
        "2024-10-16 NJC: update to be VocPub 4.10 valid" ,
        "2016-07-22 OLR: Reformat SKOS-RDF for migration to new repository" ,
        "2015-11-26: Original SKOS implementation" ;
    skos:definition "This concept scheme defines terms used to describe the type of mineral tenements granted in Australian and New Zealand jurisdictions (eg, exploration licence, mining lease)."@en ;
    skos:editorialNote "This file contains the 2015 version of the GGIC mineral temement type vocabulary. Compilation and review in MS-Excel spreadsheet, converted to SKOS using GSML_SKOS_fromXLS_2015.02.xslt."@en ;
    skos:hasTopConcept
        :exploration ,
        :production ;
    skos:prefLabel "GGIC Tenement Type"@en ;
.
